spec/design/skel/X64/Hardware_H.thy
@@ -16,7 +16,7 @@ begin
 
 context Arch begin global_naming X64_H
 
-#INCLUDE_HASKELL SEL4/Machine/Hardware/X64.lhs Platform=Platform.X64 CONTEXT X64_H NOT getMemoryRegions getDeviceRegions getKernelDevices loadWord storeWord storeWordVM getActiveIRQ ackInterrupt maskInterrupt configureTimer resetTimer debugPrint getRestartPC setNextPC clearMemory clearMemoryVM initMemory freeMemory setCurrentPD setGlobalPD setHardwareASID wordFromPDE wordFromPTE VMFaultType HypFaultType VMMapType VMPageSize pageBits pageBitsForSize toPAddr addrFromPPtr ptrFromPAddr setCurrentCR3 getCurrentCR3 invalidateTLB invalidateTLBEntry mfence wordFromPML4E wordFromPDPTE firstValidIODomain numIODomainIDBits hwASIDInvalidate getFaultAddress irqIntOffset maxPCIBus maxPCIDev maxPCIFunc numIOAPICs ioapicIRQLines ioapicMapPinToVector irqStateIRQIOAPICNew irqStateIRQMSINew updateIRQState X64IRQState in8 out8 in16 out16 in32 out32 invalidatePageStructureCache resetCR3 physBase archSetCurrentVSpaceRoot writeCR3 invalidateASID invalidateTranslationSingleASID invalidatePageStructureCacheASID ptTranslationBits
+#INCLUDE_HASKELL SEL4/Machine/Hardware/X64.lhs Platform=Platform.X64 CONTEXT X64_H NOT getMemoryRegions getDeviceRegions getKernelDevices loadWord storeWord storeWordVM getActiveIRQ ackInterrupt maskInterrupt configureTimer resetTimer debugPrint getRestartPC setNextPC clearMemory clearMemoryVM initMemory freeMemory wordFromPDE wordFromPTE VMFaultType HypFaultType VMMapType VMPageSize pageBits pageBitsForSize toPAddr addrFromPPtr ptrFromPAddr setCurrentUserCR3 getCurrentUserCR3 invalidateTLB invalidateTLBEntry mfence wordFromPML4E wordFromPDPTE firstValidIODomain numIODomainIDBits hwASIDInvalidate getFaultAddress irqIntOffset maxPCIBus maxPCIDev maxPCIFunc numIOAPICs ioapicIRQLines ioapicMapPinToVector irqStateIRQIOAPICNew irqStateIRQMSINew updateIRQState X64IRQState in8 out8 in16 out16 in32 out32 invalidatePageStructureCache writeCR3 invalidateASID invalidateTranslationSingleASID invalidateLocalPageStructureCacheASID ptTranslationBits
 
 end
 
@@ -26,7 +26,7 @@ end
 
 context Arch begin global_naming X64_H
 
-#INCLUDE_HASKELL SEL4/Machine/Hardware/X64.lhs CONTEXT X64_H instanceproofs NOT HardwareASID VMFaultType VMPageSize VMPageEntry VMMapType HypFaultType
+#INCLUDE_HASKELL SEL4/Machine/Hardware/X64.lhs CONTEXT X64_H instanceproofs NOT VMFaultType VMPageSize VMPageEntry VMMapType HypFaultType
 
 #INCLUDE_HASKELL SEL4/Machine/Hardware/X64.lhs CONTEXT X64_H ONLY wordFromPDE wordFromPTE wordFromPML4E wordFromPDPTE
 
